raft/RaftMsgRefinementInterface.v
@@ -34,11 +34,11 @@ Section RaftMsgRefinementInterface.
   Hint Extern 3 (@FailureParams _ _) => apply raft_msg_refined_failure_params : typeclass_instances.
 
   Inductive msg_refined_raft_intermediate_reachable : network -> Prop :=
-  | MRRIR_init : msg_refined_raft_intermediate_reachable step_m_init
-  | MRRIR_step_f :
+  | MRRIR_init : msg_refined_raft_intermediate_reachable step_async_init
+  | MRRIR_step_failure :
       forall failed net failed' net' out,
         msg_refined_raft_intermediate_reachable net ->
-        step_f (failed, net) (failed', net') out ->
+        step_failure (failed, net) (failed', net') out ->
         msg_refined_raft_intermediate_reachable net'
   | MRRIR_handleInput :
       forall net h inp gd out d l ps' st',
@@ -192,7 +192,7 @@ Section RaftMsgRefinementInterface.
       P net'.
 
   Definition msg_refined_raft_net_invariant_init (P : network -> Prop) :=
-    P step_m_init.
+    P step_async_init.
   
   Definition msg_refined_raft_net_invariant_client_request' (P : network -> Prop) :=
     forall h net st' ps' gd out d l client id c,
